---
layout: note
title:  "Haskell: Higher-order Functions"
date:   2021-02-05 09:34:44 -0600
categories: csce 314
semester: spring21
---

## Higher Order Functions
A function is considered to be higher-order if it takes a function as an argument or returns a funciton as a result.

```haskell
twice :: (a -> a) -> a -> a
twice f x = f (f x)
```

- Common programming idioms can be encoded as afunctions
- Domain specific languages can be defined as collections of higher-order functions (e.g. for processing lists)
- Algebraic properties of higher-order functions can be used to reason about programs

## map
- map applies a function to every element of a list

```haskell
map :: (a -> b) -> [a] -> [b]

> map (+1) [1,3,5,7]
[2,4,6,8]
```

## filter
- filter selects every element from a list that satisfies a predicate

```haskell
filter :: (a -> Bool) -> [a] -> [a]

> filter even [1..10]
[2,4,6,8,10]
```

- filter can be defined using a list comprehension

```haskell
filter p xs = [x | xs <- xs, p x]
```

- alternatively, through recursion

```haskell
filter p [] = []
filter p (x:xs)
    | p x       = x : filter p xs
    | otherwise = filter p xs
```

## foldr
- many functions can be defined using a simple pattern of recursion, which can then be expressed as folding to the right.

```haskell
f [] = v -- v is base value
f (x:xs) = x # f xs ]
    -- any non-empty list to some function # to its head, and f of its tail
-- any empty list gets mapped to v
```

- sum
    ```haskell
    sum [] = 0
    sum (x:xs) = x + sum xs

    sum = foldr (+) 0
    ```
- product
    ```haskell
    product [] = 1
    product (x:xs) = x * product xs

    product = foldr (*) 1
    ```
- and
    ```haskell
    and [] = True
    and (x:xs) = x && and xs

    and = foldr (&&) True
    ```

foldr can be defined using recursion

```haskell
foldr :: (a -> b -> b) -> b -> [a] -> b
foldr f v [] = v
foldr f v (x:xs) = f x (foldr f v xs)
```

However, it could help to think of folder as replacing every cons operator in a list with the given function, and the empty list with the base value.

```haskell
length :: [a] -> Int
length [] = 0
length (_:xs) = 1 + length xs
```
